First we split the sum $\sum_{k=0}^{n} \binom{-t+k}{j}$ into two sub-sums so that we discuss them separately
\begin{align*}
    \sum_{k=0}^{n} \binom{-t+k}{j} &= \sum_{k=0}^{t-1} \binom{-t+k}{j} + \sum_{k=t}^{n} \binom{-t+k}{j}
\end{align*}
We assume that the two sums above run over the partition $\{0,1,2,\cdots,t,\cdots, n\}$ such that $t<n$.
Considering the sum $\sum_{k=0}^{t-1} \binom{-t+k}{j}$ we notice that
\begin{align*}
    \sum_{k=0}^{t-1} \binom{-t+k}{j} = \binom{-t}{j}
    &+ \binom{-t +1}{j} + \binom{-t+2}{j} + \cdots + \\
    &+ \binom{-t+t-2}{j} + \binom{-t+t-1}{j}
\end{align*}
Thus
\begin{align*}
    \sum_{k=0}^{t-1} \binom{-t+k}{j} &= \sum_{k=1}^{t} \binom{-k}{j} = \sum_{k=0}^{t-1} \binom{-k-1}{j}
\end{align*}
By means of $\binom{-k}{j} = (-1)^j \binom{j+k-1}{j}$
\begin{align*}
    \binom{-k-1}{j} &= \binom{-(k+1)}{j} = (-1)^j \binom{j+k}{j}
\end{align*}
Thus
\begin{align*}
    \sum_{k=0}^{t-1} \binom{-t+k}{j} = (-1)^j \sum_{k=0}^{t-1} \binom{j+k}{j} = (-1)^{j} \binom{j+t}{j+1}
\end{align*}
By means of Hockey stick identity $\sum_{k=0}^{t} \binom{j+k}{j} = \binom{j+t+1}{j+1}$.

Considering the sum $\sum_{k=t}^{n} \binom{-t+k}{j}$ we notice that
\begin{align*}
    \sum_{k=t}^{n} \binom{-t+k}{j} = \sum_{k=0}^{n-t} \binom{k}{j}
\end{align*}
Thus
\begin{align*}
    \sum_{k=t}^{n} \binom{-t+k}{j} = \sum_{k=0}^{n-t} \binom{k}{j} = \binom{n-t+1}{j+1}
\end{align*}
By means of Hockey stick identity $\sum_{k=0}^{t} \binom{j+k}{j} = \binom{j+t+1}{j+1}$.
Thus
\begin{align*}
    \sum_{k=0}^{n} \binom{-t+k}{j} &= (-1)^j \binom{j+t}{j+1} +  \binom{n-t+1}{j+1}
\end{align*}
This completes the proof.
